

3-1-3.

$$y = C_1 x + C_2 x \ln x. \quad (0, \infty); \quad x^2 y'' - x y' + y = 0. \quad y(1) = 3, \quad y'(1) = -1.$$

$$y' = C_1 + C_2(1 + \ln x) = C_1 + C_2 + C_2 \ln x$$

$$y'' = \frac{C_2}{x}. \quad x^2 \cdot \frac{C_2}{x} - x(C_1 + C_2 + C_2 \ln x) + y = 0.$$

$$(2x - xC_1 - xC_2 - xC_2 \ln x) + y = y - xC_1 - xC_2 \ln x = 0.$$

$$y = xC_1 + xC_2 \ln x.$$

$$C_1 = 3. \quad 3 + C_2 = -1 \quad C_2 = -4. \quad y = 3x - 4x \ln x.$$

3-1-13.

$$y = C_1 e^x \cos x + C_2 e^x \sin x. \quad y'' - 2y' + 2y = 0.$$

$$(a) \quad y = e^x (C_1 \cos x + C_2 \sin x). \quad y' = e^x (C_1 \cos x + C_2 \sin x) + e^x (C_2 \cos x - C_1 \sin x)$$

$$y'(\pi) = e^\pi (C_1 (\cos \pi - \sin \pi) + C_2 (\sin \pi + \cos \pi)) = -e^\pi (C_1 + C_2) = 0. \quad C_1 + C_2 = 0.$$

$$y(0) = e^0 (C_1) = 1. \quad C_1 = 1. \quad C_2 = -1. \quad \rightarrow \text{가능}$$

$$(b) \quad C_1 = 1. \quad y(\pi) = e^\pi (C_1 \cos \pi + C_2 \sin \pi) = e^\pi. \quad -C_1 = -e^\pi \rightarrow \text{불가능}$$

$$(c) \quad C_1 = 1. \quad y\left(\frac{\pi}{2}\right) = e^{\frac{\pi}{2}} (C_1 \cos \frac{\pi}{2} + C_2 \sin \frac{\pi}{2}) = e^{\frac{\pi}{2}} (0 + C_2) = e^{\frac{\pi}{2}} C_2$$

$$C_2 = \frac{1}{e^{\frac{\pi}{2}}} \rightarrow \text{가능}$$

$$(d) \quad C_1 = 0. \quad y(\pi) = e^\pi (C_1 \cos \pi + C_2 \sin \pi) = e^\pi C_2 = 0. \rightarrow \text{가능}$$

3-1-17.

$$f(x) = 5, \quad f_1(x) = \cos^2 x, \quad f_2(x) = \sin^2 x.$$

$$5(\cos^2 x + \sin^2 x) = f(x). \quad f_1(x) = 5f_2(x) + 5f_3(x) \rightarrow \text{만족}$$

3-1-25.

$$y'' - 2y' + 5y = 0. \quad e^x \cos 2x, \quad e^x \sin 2x, \quad (-\infty, \infty)$$

$$r^2 - 2r + 5 = 0. \quad 1 \pm 2i = r. \quad e^{ix} = \cos x + i \sin x. \quad y(x) = C_1 e^{(1+2i)x} + C_2 e^{(1-2i)x}$$

$$e^{(1+2i)x} = e^x (\cos 2x + i \sin 2x). \quad e^{(1-2i)x} = e^x (\cos 2x - i \sin 2x)$$

$$y(x) = C_1 e^x \cos 2x + C_2 e^x \sin 2x$$

3-1-33.

$$y'' - 4y' + 4y = 2e^{2x} + 4x - 12; \quad y = C_1 e^{2x} + C_2 x e^{2x} + x^2 e^{2x} + x - 2.$$

$$r^2 - 4r + 4 = 0. \quad r = 2. \quad y_1(x) = C_1 e^{2x} + C_2 x e^{2x}. \quad y_2(x) = A x^2 e^{2x} + B x + C.$$

$$y = C_1 e^{2x} + C_2 x e^{2x} + x^2 e^{2x} + x - 2.$$

3-2-1.

$$r^2 - 4r + 4 = 0. \quad r = 2. \quad y = C_1 e^{2x} + C_2 x e^{2x}. \quad y_2 = x e^{2x}.$$

3-2-7.

$$9r^2 - 12r + 4 = 0. \quad r = \frac{2}{3}. \quad y = C_1 e^{\frac{2}{3}x} + C_2 x e^{\frac{2}{3}x}. \quad y_2 = x e^{\frac{2}{3}x}.$$

$$\frac{2}{3} \quad -\frac{2}{3}$$

3-3-1.

$$4r^2 + r = 0. \quad r(4r+1) \quad r = 0, -\frac{1}{4}$$

$$y(x) = C_1 + C_2 e^{-\frac{1}{4}x}$$

3-3-5.

$$r^2 + 8r + 16 = 0. \quad r = -4. \quad y(x) = C_1 e^{-4x} + C_2 x e^{-4x}.$$

3-3-11.

$$r^2 - 4r + 5 = 0. \quad r = 2, i. \quad y(x) = C_1 e^x + C_2 e^{ix}$$

$$\frac{5}{-1}$$

3-3-15.

$$r(r^2 - 4r - 5) = 0. \quad r = 0, 1, 5. \quad y(x) = C_1 + C_2 e^x + C_3 e^{5x}$$

$$\frac{5}{-1}$$

3-3-19.

$$r^4 + r^2 - 2r = 0. \quad r(r^3 + r - 2) = 0. \quad r = 0, 1, -2.$$

$$y(x) = C_1 + C_2 e^{-x} + C_3 e^{-2x}.$$

3-3-31.

$$y'' + 16y = 0. \quad y(0) = 2, \quad y'(0) = -2.$$

$$r^2 + 16r = 0. \quad r = 0, -16. \quad y(x) = C_1 + C_2 e^{-16x}. \quad C_1 + C_2 = 2. \quad y'(x) = -16C_2 e^{-16x}$$

$$-16C_2 = -2 \quad C_2 = \frac{1}{8}. \quad C_1 = \frac{15}{8}. \quad y(x) = \frac{15}{8} + \frac{1}{8} e^{-16x}.$$

3-3-37.

$$r^3 + 12r^2 + 36r = 0. \quad r(r^2 + 12r + 36) = 0. \quad r = 0, -6$$

$$y(x) = C_1 + C_2 e^{-6x} + C_3 x e^{-6x}. \quad y'(x) = -6C_2 e^{-6x} + C_3 e^{-6x} - 6C_3 x e^{-6x}.$$

$$y''(x) = 36C_2 e^{-6x} - 12C_3 e^{-6x} + 36C_3 x e^{-6x}. \quad C_1 = -C_2. \quad -6C_2 + C_3 = 1.$$

$$36C_2 - 12C_3 = -1. \quad 36C_2 - 12(C_2 + 1) = -1. \quad 36C_2 - 12C_2 - 12 = -1.$$

$$-36C_2 = 11 \quad C_2 = -\frac{11}{36}. \quad C_3 = 6x - \frac{5}{36} + 1 = \frac{1}{6}.$$

$$y(x) = \frac{11}{36} - \frac{11}{36} e^{-6x} + \frac{1}{6} x e^{-6x}.$$

3-4.3.

$$y'' - 10y' + 25y = 30x + 3, \quad r^2 - 10r + 25 = 0, \quad r = 5. \quad (3)$$

$$y_h(x) = C_1 e^{5x} + C_2 x e^{5x}, \quad y_p(x) = Ax + B, \quad y_p' = A, \quad y_p'' = 0.$$

$$0 - 10A + 25(Ax + B) = 30x + 3, \quad 25A = 30, \quad A = \frac{6}{5}, \quad B = \frac{3}{5}.$$

$$y(x) = C_1 e^{5x} + C_2 x e^{5x} + \frac{6}{5}x + \frac{3}{5}.$$

3-4.13.

$$y'' + 4y = 3 \sin 2x, \quad r^2 + 4 = 0, \quad r = \pm 2i.$$

$$y_h(x) = C_1 \cos 2x + C_2 \sin 2x, \quad (x) \quad r = \pm 2i, \quad y_h(x) = C_1 \cos 2x + C_2 \sin 2x.$$

$$y_p = x(A \cos 2x + B \sin 2x).$$

$$y_p' = A \cos 2x + B \sin 2x + x(-2A \sin 2x + 2B \cos 2x).$$

$$= A \cos 2x + B \sin 2x - 2Ax \sin 2x + 2Bx \cos 2x.$$

$$y_p'' = (-2A \sin 2x + 2B \cos 2x) + (-2A \sin 2x - 4Ax \cos 2x) + (2B \cos 2x - 4Bx \sin 2x).$$

$$y_p'' = -4A \sin 2x - 4Bx \sin 2x + 4B \cos 2x - 4Ax \cos 2x.$$

$$4y_p = 4x(A \cos 2x + B \sin 2x), \quad y_p'' + 4y_p = -4A \sin 2x + 4B \cos 2x.$$

$$3 \sin 2x + 0 \cos 2x, \quad A = -\frac{3}{4}, \quad B = 0.$$

$$y(x) = C_1 \cos 2x + C_2 \sin 2x - \frac{3}{4}x \cos 2x.$$

3-4.17.

$$r^2 - 2r + 5 = 0, \quad r = \frac{2 \pm 4i}{2} = 1 \pm 2i$$

$$y_h = C_1 e^{(1+2i)x} + C_2 e^{(1-2i)x}, \quad y_p = x e^x (A \cos 2x + B \sin 2x)$$

$$y_p' = e^x (A \cos 2x + B \sin 2x) + x e^x (A \cos 2x + B \sin 2x) + x e^x (-2A \sin 2x + 2B \cos 2x)$$

$$y_p'' = e^x (A \cos 2x + B \sin 2x) + x e^x [(A \cos 2x + B \sin 2x) + (2B \cos 2x - 2A \sin 2x)]$$

$$= e^x (A \cos 2x + B \sin 2x) + x e^x [(A + 2B) \cos 2x + (2B - 2A) \sin 2x]$$

$$y'' - 2y' + 5y = e^x [(C_1 \cos 2x + C_2 \sin 2x)] \Rightarrow C_1 = 1, C_2 = 0, \quad A = 0, B = \frac{1}{10}.$$

$$\therefore y(x) = C_1 e^x \cos 2x + C_2 e^x \sin 2x + \frac{1}{10} x e^x \sin 2x.$$

3-4.21.

$$r^2 + 4r + 5 = 0, \quad r = \frac{-4 \pm \sqrt{16-20}}{2} = -2 \pm i$$

$$y_h(x) = e^{-2x} (C_1 \cos x + C_2 \sin x), \quad y_p = A e^{-4x}, \quad y_p' = -4A e^{-4x}.$$

$$y_p'' = 16A e^{-4x}, \quad 16A e^{-4x} - 16A e^{-4x} + 5A e^{-4x} = 5A e^{-4x}, \quad A = 1.$$

$$y_p = e^{-4x}, \quad y(x) = e^{-2x} (C_1 \cos x + C_2 \sin x) + e^{-4x}, \quad y(0) = -3.$$

$$y(0) = C_1 + C_2 + 1 = C_1 + 1 = -3, \quad C_1 = -10.$$

$$y'(x) = e^{-2x} (-2)(C_1 \cos x + C_2 \sin x) + (-C_1 \sin x + C_2 \cos x)$$

$$= e^{-2x} (-2C_1 \cos x - 2C_2 \sin x - C_1 \sin x + C_2 \cos x) - 2B e^{-4x}.$$

$$y'(0) = (-2C_1 - C_2 + C_2) = -2C_1 = -2(-10) = 20.$$

$$20 - C_2 - 2B = -C_2 - 2 = 20, \quad C_2 = -22.$$

$$\therefore y(x) = e^{-2x} (-10 \cos x - 22 \sin x) + e^{-4x}.$$

3-4.21.

$$y'' + y = x^2 + 1, \quad y(0) = 5, \quad y(\pi) = 0, \quad r^2 + 1 = 0, \quad r = \pm i.$$

$$y_h = C_1 \cos x + C_2 \sin x, \quad y_p = Ax^2 + Bx + C, \quad y_p' = 2Ax.$$

$$2A(Ax^2 + Bx + C) = Ax^2 + Bx + 2A + C = x^2 + 1, \quad A = 1, B = 0, 2A + C = 1.$$

$$C = -1, \quad y_p = x^2 - 1.$$

$$y(x) = C_1 \cos x + C_2 \sin x + x^2 - 1, \quad y(0) = 5, \quad C_1 - 1 = 5, \quad C_1 = 6.$$

$$y(\pi) = C_1 \cos \pi + C_2 \sin \pi + \pi^2 - 1 = 0, \quad 6 \cos \pi + C_2 \sin \pi = 0, \quad \dots ?$$

$$C_2 = \frac{-3.241}{0.8415} \approx -3.85 \Rightarrow -\frac{6 \cos 1}{\sin 1}$$

$$y(x) = 6 \cos x - 3.85 \sin x + x^2 - 1.$$

3-5.1

$$y'' + y = \sec x, \quad r^2 + 1 = 0, \quad r = \pm i, \quad y_h = C_1 \cos x + C_2 \sin x.$$

$$y_p = u_1 \cos x + u_2 \sin x.$$

$$u_1' \cos x - u_2' \sin x = 0.$$

$$-u_1' \sin x + u_2' \cos x = \sec x, \quad u_1' = -u_2' \frac{\sin x}{\cos x} = -u_2' \tan x.$$

$$-(-u_2' \tan x) \sin x + u_2' \cos x = \sec x, \quad u_2' \tan x \sin x + u_2' \cos x = \sec x.$$

$$u_2' \tan x \sin x + u_2' \cos x = \sec x, \quad u_2' \left(\frac{\sin^2 x}{\cos x} + \cos x \right) = \sec x.$$

$$u_2' \left(\frac{\sin^2 x + \cos^2 x}{\cos x} \right) = \sec x, \quad u_2' = \cos x \sec x = 1, \quad u_1' = \tan x.$$

$$u_1 = \int u_1' dx = \int \tan x dx = -\ln |\cos x| + C_1.$$

$$u_2 = \int u_2' dx = \int 1 dx = x + C_2, \quad y_p = u_1 \cos x + u_2 \sin x$$

$$= (-\ln |\cos x|) \cos x + x \sin x.$$

$$y(x) = C_1 \cos x + C_2 \sin x - \ln |\cos x| \cos x + x \sin x.$$

3-5.11.

$$r^2 - 1 = 0, \quad r = \pm 1, \quad y_h = C_1 e^x + C_2 e^{-x}$$

$$y_p = u_1 e^x + u_2 e^{-x}.$$

$$u_1' e^x + u_2' e^{-x} = 0.$$

$$u_1' e^x - u_2' e^{-x} = \cosh x, \quad 2u_1' e^x = \cosh x, \quad u_1' = \frac{\cosh x}{2e^x}.$$

$$2u_2' e^{-x} = -\cosh x, \quad u_2' = -\frac{\cosh x}{2e^{-x}} = -\frac{\cosh x \cdot e^x}{2}.$$

$$u_1 = \frac{1}{2} \int \frac{e^x + e^{-x}}{2e^x} dx = \frac{1}{2} \int \left(\frac{1}{2} + \frac{e^{-2x}}{2} \right) dx = \frac{1}{4} x - \frac{1}{8} e^{-2x}.$$

$$u_2 = -\frac{1}{2} \int (\cosh x) dx = -\frac{1}{2} \int \left(\frac{e^x + e^{-x}}{2} \right) dx = -\frac{1}{4} \int (e^x + e^{-x}) dx = -\frac{1}{4} \left(\frac{e^x}{1} + \frac{e^{-x}}{-1} \right) = -\frac{1}{4} (e^x - e^{-x}).$$

$$y_p = \left(\frac{x}{4} - \frac{1}{8} e^{-2x} \right) e^x + \left(-\frac{1}{4} (e^x - e^{-x}) \right) e^{-x} = \frac{x}{4} (e^x - e^{-x}) - \frac{1}{8} (e^x + e^{-x}).$$

$$y(x) = C_1 e^x + C_2 e^{-x} + \frac{x}{4} (e^x - e^{-x}) - \frac{1}{8} (e^x + e^{-x}).$$

25.21.

$$4y'' - y = xe^{\frac{x}{2}}, \quad y(0)=1, \quad y'(0)=0.$$

$$y' - \frac{1}{4}y = \frac{1}{4}xe^{\frac{x}{2}}, \quad r^2 - \frac{1}{4} = 0, \quad r = \pm \frac{1}{2}, \quad y_h = C_1 e^{\frac{x}{2}} + C_2 e^{-\frac{x}{2}}.$$

$$y_p = u_1 e^{\frac{x}{2}} + u_2 e^{-\frac{x}{2}}.$$

$$u_1' e^{\frac{x}{2}} + u_2' e^{-\frac{x}{2}} = 0.$$

$$u_1' \cdot \frac{1}{2} e^{\frac{x}{2}} - u_2' \cdot \frac{1}{2} e^{-\frac{x}{2}} = \frac{1}{4} x e^{\frac{x}{2}}, \quad u_1' = -u_2' e^{-x}.$$

$$\frac{1}{2} (-u_2' e^{-x}) e^{\frac{x}{2}} - \frac{1}{2} u_2' e^{-\frac{x}{2}} = \frac{1}{4} x e^{\frac{x}{2}}, \quad -u_2' e^{-\frac{x}{2}} = \frac{1}{4} x e^{\frac{x}{2}}, \quad u_2' = -\frac{1}{4} x e^{x}.$$

$$u_1' = -u_2' e^{-x} = \left(\frac{1}{4} x e^x\right) e^{-x} = \frac{1}{4} x.$$

$$u_1 = \frac{1}{8} x^2, \quad u_2 = -\frac{1}{4} \cdot \frac{1}{4} (x e^x - \int e^x dx) = -\frac{1}{4} (x e^x - e^x) = -\frac{1}{4} e^x (x-1)$$

$$y_p = \left(\frac{1}{8} x^2\right) e^{\frac{x}{2}} + \left(-\frac{1}{4} e^x (x-1)\right) e^{-\frac{x}{2}} = \left(\frac{1}{8} x^2 - \frac{1}{4} x + \frac{1}{4}\right) e^{\frac{x}{2}}.$$

$$y(x) = C_1 e^{\frac{x}{2}} + C_2 e^{-\frac{x}{2}} + \left(\frac{1}{8} x^2 - \frac{1}{4} x + \frac{1}{4}\right) e^{\frac{x}{2}}, \quad y(0)=1, \quad C_1 + C_2 + \frac{1}{4} = 1, \quad C_1 + C_2 = \frac{3}{4}.$$

$$y'(x) = \frac{1}{2} C_1 e^{\frac{x}{2}} - \frac{1}{2} C_2 e^{-\frac{x}{2}} + \left(\frac{1}{4} x - \frac{1}{2}\right) e^{\frac{x}{2}}, \quad y'(0)=0, \quad \frac{1}{2} C_1 - \frac{1}{2} C_2 + \frac{1}{4} = 0, \quad C_1 - C_2 = -\frac{1}{2}.$$

$$y'(0) = -\frac{1}{4} + \left(C_1 + \frac{1}{4}\right) \cdot \frac{1}{2} - \frac{1}{2} C_2 = \frac{C_1 - C_2}{2} - \frac{1}{4} = 0, \quad C_1 - C_2 = \frac{1}{2}.$$

$$C_1 = \frac{1}{2}, \quad C_2 = \frac{1}{4}, \quad y(x) = \left(\frac{1}{2} + \frac{1}{8} x^2 - \frac{1}{4} x + \frac{1}{4}\right) e^{\frac{x}{2}} + \frac{1}{4} e^{-\frac{x}{2}}$$

25.23.

$$r^2 - 2r + 1 = 0, \quad r = 1 \quad (\text{중근}). \quad y_h = C_1 e^x + C_2 x e^x, \quad y_p = u_1 e^x + u_2 x e^x.$$

$$u_1' e^x + u_2' x e^x = 0.$$

$$u_1' e^x + u_2' (x+1) e^x = e^x \sec^2 x, \quad u_1' = -u_2' x.$$

$$-u_2' x + u_2' (x+1) = \sec^2 x, \quad u_2' = \sec^2 x, \quad u_1' = -x \sec^2 x.$$

$$u_2 = \int \sec^2 x dx = \tan x, \quad u_1 = -\int x \sec^2 x dx = -x \tan x + \ln |\cos x|$$

$$y_p = u_1 e^x + u_2 x e^x = (-x \tan x + \ln |\cos x|) e^x + x \tan x e^x = \ln |\cos x| \cdot e^x.$$

$$y(x) = C_1 e^x + C_2 x e^x + \ln |\cos x| \cdot e^x, \quad y(0)=1, \quad C_1 = 1.$$

$$y'(x) = e^x (C_1 + C_2 x + \ln |\cos x|)' + e^x (C_1 + C_2 x + \ln |\cos x|).$$

$$= e^x (C_2 - \tan x + C_1 + C_2 x + \ln |\cos x|), \quad x=0, \quad \tan 0=0, \quad \ln 1=0.$$

$$y'(0) = C_1 + C_2 = 1 + C_2 = 0, \quad C_2 = -1, \quad y(x) = e^x (1 - x + \ln |\cos x|).$$